DistributedSystems/VerifiedDS/src/Dafny/Distributed/Protocol/CausalMesh/proof/read_deps_is_met.dfy
@@ -1,0 +1,40 @@
+include "../distributed_system.dfy"
+// include "causalcut.dfy"
+include "packet_sending.dfy"
+include "properties.dfy"
+include "read_reply_is_met.dfy"
+include "../../../Common/Collections/Seqs.s.dfy"
+
+module CausalMesh_Proof_ReadDepsIsMet_i {
+import opened CausalMesh_Cache_i
+import opened CausalMesh_Message_i
+import opened CausalMesh_Types_i
+import opened Environment_s
+import opened CausalMesh_DistributedSystem_i
+import opened CausalMesh_Properties_i
+import opened CausalMesh_PullDeps_i
+import opened CausalMesh_Proof_Actions_i
+import opened Temporal__Temporal_s
+import opened CausalMesh_proof_Assumptions_i
+import opened CausalMesh_Proof_Constants_i
+import opened CausalMesh_Proof_PacketSending_i
+import opened CausalMesh_Proof_Properties_i
+import opened CausalMesh_Proof_DepsAreMet_i
+import opened CausalMesh_Proof_ReadReplyIsMet_i
+import opened Collections__Seqs_s
+import opened Collections__Maps_i
+import opened Collections__Maps2_s
+
+lemma lemma_ReadDepsIsMetPrefix(
+    b:Behavior<CMState>,
+    i:int
+)
+    requires 0 < i 
+    requires IsValidBehaviorPrefix(b, i)
+    requires CMNext(b[i-1], b[i])
+    decreases i
+{
+
+}
+
+}
